src/codegen/extraction.v
@@ -2,7 +2,6 @@ Require Import ExtrOcamlBasic.
 Require Import ExtrOcamlString.
 Require Import ExtrOcamlNatInt.
 Require Import DiskLog.
-Require Import MemLog.
 Require Import Trans.
 Require Import Bank.
 Require Import Storage.
@@ -11,7 +10,6 @@ Extraction Blacklist List String Int.
 
 Cd "codegen".
 Extraction Library DiskLog.
-Extraction Library MemLog.
 Extraction Library Trans.
 Extraction Library Bank.
 Extraction Library Storage.
